fill in map summation proofs

concurrency/scache/FullMap.i.dfy
@@ -1,43 +1,166 @@
+include "MapSum.i.dfy"
+
 module FullMaps {
+  export S provides HasFiniteSupport, SumFilter, SumFilterSimp, UseZeroSum,
+              lemma_zero_map_finite_support, lemma_unit_fn_finite_support,
+              lemma_add_fns_finite_support
+           reveals IsFull, FullMap, zero_map, unit_fn, add_fns,
+                  zero_map_internal, unit_fn_internal, add_fns_internal
+  export extends S
+
+  import MapSum
+
   predicate IsFull<K(!new), V>(m: imap<K, V>) {
     forall k :: k in m
   }
 
-  type FullMap<K(!new), V> = m : imap<K, V> | IsFull(m)
+  predicate IsFiniteSupport<K(!new)>(m: imap<K, nat>, finite_map: map<K, nat>)
+  {
+    forall k ::
+      && (k in finite_map ==> k in m && m[k] == finite_map[k])
+      && (k in m && m[k] != 0 ==> k in finite_map)
+  }
+
+  predicate HasFiniteSupport<K(!new)>(m: imap<K, nat>)
+  {
+    exists finite_map :: IsFiniteSupport(m, finite_map)
+  }
+
+  type FullMap<K(!new,==)> = m : imap<K, nat> | IsFull(m) && HasFiniteSupport(m)
     witness *
 
-  function zero_map<A(!new)>() : imap<A, nat> {
+  function GetFiniteSupport<K(!new)>(m: FullMap<K>) : map<K, nat>
+  requires HasFiniteSupport(m)
+  {
+    var finite_map :| IsFiniteSupport(m, finite_map); finite_map
+  }
+
+  function zero_map_internal<K(!new)>() : imap<K, nat> {
     imap k {:trigger} | true :: 0
   }
 
-  function unit_fn<A(!new)>(a: A) : FullMap<A, nat> {
+  lemma lemma_zero_map_finite_support<K(!new)>()
+  ensures var k: imap<K, nat> := zero_map_internal();
+    HasFiniteSupport(k);
+  {
+    var k: imap<K, nat> := zero_map_internal();
+    assert IsFiniteSupport(k, map[]);
+  }
+
+  function zero_map<K(!new)>() : FullMap<K> {
+    lemma_zero_map_finite_support<K>();
+    imap k {:trigger} | true :: 0
+  }
+
+  function unit_fn_internal<K(!new)>(a: K) : imap<K, nat> {
     imap k {:trigger} | true :: (if k == a then 1 else 0)
   }
 
-  function add_fns<A(!new)>(f: FullMap<A, nat>, g: FullMap<A, nat>) : FullMap<A, nat> {
+  lemma lemma_unit_fn_finite_support<K(!new)>(a: K)
+  ensures HasFiniteSupport(unit_fn_internal(a))
+  {
+    assert IsFiniteSupport(unit_fn_internal(a), map[a := 1]);
+  }
+
+  function unit_fn<K(!new)>(a: K) : FullMap<K> {
+    lemma_unit_fn_finite_support(a);
+    unit_fn_internal(a)
+  }
+
+  function add_fns_internal<K(!new)>(f: FullMap<K>, g: FullMap<K>) : imap<K, nat> {
     imap b | true :: f[b] + g[b]
   }
 
-  function SumFilter<A(!new)>(fn: (A) -> bool, f: FullMap<A, nat>) : nat
+  lemma lemma_add_fns_finite_support<K(!new)>(f: FullMap<K>, g: FullMap<K>)
+  ensures HasFiniteSupport(add_fns_internal(f, g))
+  {
+    var a := GetFiniteSupport(f);
+    var b := GetFiniteSupport(g);
 
-  lemma SumFilterSimp<A>()
-  ensures forall fn: (A) -> bool, f: FullMap<A, nat>, g: FullMap<A, nat>
+    assert IsFiniteSupport(add_fns_internal(f, g),
+        map k | k in a.Keys + b.Keys :: add_fns_internal(f, g)[k]);
+  }
+
+  function add_fns<K(!new)>(f: FullMap<K>, g: FullMap<K>) : FullMap<K> {
+    lemma_add_fns_finite_support(f, g);
+    add_fns_internal(f, g)
+  }
+
+  function Filter<K(!new)>(fn: (K) -> bool, m: map<K, nat>) : map<K, nat> {
+    map k | k in m.Keys && fn(k) :: m[k]
+  }
+
+  function SumFilter<K(!new)>(fn: (K) -> bool, f: FullMap<K>) : nat
+  requires HasFiniteSupport(f)
+  {
+    MapSum.Sum(Filter(fn, GetFiniteSupport(f)))
+  }
+
+  lemma SumFilterAdditive<K(!new)>(fn: (K) -> bool, f: FullMap<K>, g: FullMap<K>)
+  ensures SumFilter(fn, add_fns(f, g)) == SumFilter(fn, f) + SumFilter(fn, g)
+  {
+    MapSum.SumAdditive(Filter(fn, GetFiniteSupport(add_fns(f, g))),
+        Filter(fn, GetFiniteSupport(f)),
+        Filter(fn, GetFiniteSupport(g)));
+  }
+
+  lemma SumFilterSingle<K(!new)>(fn: (K) -> bool, x: K)
+  ensures SumFilter(fn, unit_fn(x)) == (if fn(x) then 1 else 0)
+  {
+    var f := Filter(fn, GetFiniteSupport(unit_fn(x)));
+    if fn(x) {
+      var f1 := f - {x};
+      assert f1[x := f[x]] == f;
+      MapSum.SumAllZeroesIsZero(f1);
+      MapSum.SumInduct(f1, x, f[x]);
+    } else {
+      MapSum.SumAllZeroesIsZero(f);
+    }
+  }
+
+  lemma SumFilterSimp<K(!new)>()
+  ensures forall fn: (K) -> bool, f: FullMap<K>, g: FullMap<K>
       {:trigger SumFilter(fn, add_fns(f, g)) } ::
       SumFilter(fn, add_fns(f, g)) == SumFilter(fn, f) + SumFilter(fn, g)
 
-  ensures forall fn: (A) -> bool, x: A
+  ensures forall fn: (K) -> bool, x: K
       {:trigger SumFilter(fn, unit_fn(x)) } ::
       SumFilter(fn, unit_fn(x)) == (if fn(x) then 1 else 0)
 
-  ensures forall fn: (A) -> bool
+  ensures forall fn: (K) -> bool
       {:trigger SumFilter(fn, zero_map()) } ::
       SumFilter(fn, zero_map()) == 0
   {
+    forall fn: (K) -> bool, f: FullMap<K>, g: FullMap<K>
+      ensures SumFilter(fn, add_fns(f, g)) == SumFilter(fn, f) + SumFilter(fn, g)
+    {
+      SumFilterAdditive(fn, f, g);
+    }
+
+    forall fn: (K) -> bool, x: K
+    ensures SumFilter(fn, unit_fn(x)) == (if fn(x) then 1 else 0)
+    {
+      SumFilterSingle(fn, x);
+    }
+
+    forall fn: (K) -> bool
+    ensures SumFilter(fn, zero_map()) == 0
+    {
+      var f := Filter(fn, GetFiniteSupport(zero_map()));
+      MapSum.SumAllZeroesIsZero(f);
+    }
   }
 
-  lemma UseZeroSum<A(!new)>(fn: (A) -> bool, f: FullMap<A, nat>)
+  lemma UseZeroSum<K(!new)>(fn: (K) -> bool, f: FullMap<K>)
+  requires HasFiniteSupport(f)
   requires SumFilter(fn, f) == 0
   ensures forall x :: fn(x) ==> f[x] == 0
   {
+    forall x | fn(x) && f[x] != 0 ensures false {
+      var m := Filter(fn, GetFiniteSupport(f));
+      var m1 := m - {x};
+      assert m1[x := m[x]] == m;
+      MapSum.SumInduct(m1, x, m[x]);
+    }
   }
 }
