concurrency/scache/MapSum.i.dfy
@@ -1,0 +1,112 @@
+module MapSum {
+  function Choose<K(!new)>(m: map<K, nat>) : K
+  requires m != map[]
+  {
+    var k :| k in m.Keys; k
+  }
+
+  function Sum<K(!new)>(m: map<K, nat>) : nat
+  {
+    if m == map[]
+      then 0
+      else (
+        var k := Choose(m);
+        Sum(m - {k}) + m[k]
+      )
+  }
+
+  lemma SumInduct<K(!new)>(m: map<K, nat>, k: K, n: nat)
+  requires k !in m
+  ensures Sum(m[k := n]) == Sum(m) + n
+  decreases |m|
+  {
+    assert m[k := n] != map[] by {
+      assert k in m[k := n];
+      var empty_map: map<K, nat> := map[];
+      assert k !in empty_map;
+    }
+    var c := Choose(m[k := n]);
+    if c == k {
+      assert m[k := n] - {k} == m;
+    } else {
+      calc {
+        Sum(m[k := n]);
+        Sum(m[k := n] - {c}) + m[k := n][c];
+        Sum(m[k := n] - {c}) + m[c];
+        { assert m[k := n] - {c} == (m - {c})[k := n]; }
+        Sum((m - {c})[k := n]) + m[c];
+        {
+          assert m == (m - {c})[c := m[c]];
+          assert |m| == |m - {c}| + 1;
+          assert |m - {c}| < |m|;
+          SumInduct(m - {c}, k, n);
+        }
+        Sum(m - {c}) + n + m[c];
+        {
+          SumInduct(m - {c}, c, m[c]);
+          assert (m - {c})[c := m[c]] == m;
+        }
+        Sum(m) + n;
+      }
+    }
+  }
+
+  lemma SumAllZeroesIsZero<K(!new)>(p: map<K, nat>)
+  requires forall k | k in p :: p[k] == 0
+  ensures Sum(p) == 0
+  {
+    if p == map[] {
+    } else {
+      var k := Choose(p);
+      SumInduct(p - {k}, k, 0);
+      assert (p - {k})[k := 0] == p;
+      SumAllZeroesIsZero(p - {k});
+    }
+  }
+
+  function GetOrZero<K(!new)>(m: map<K, nat>, k: K) : nat {
+    if k in m then m[k] else 0
+  }
+
+  lemma SumAdditive<K(!new)>(m: map<K, nat>, p: map<K, nat>, q: map<K, nat>)
+  requires forall k ::
+    GetOrZero(p, k) + GetOrZero(q, k) == GetOrZero(m, k)
+  ensures Sum(m) == Sum(p) + Sum(q)
+  {
+    if m == map[] {
+      assert forall k | k in p :: GetOrZero(p, k) == 0 ==> p[k] == 0;
+      assert forall k | k in q :: GetOrZero(q, k) == 0 ==> q[k] == 0;
+      SumAllZeroesIsZero(p);
+      SumAllZeroesIsZero(q);
+      assert Sum(m) == Sum(p) + Sum(q);
+    } else {
+      var k := Choose(m);
+      var m1 := m - {k};
+      var p1 := p - {k};
+      var q1 := q - {k};
+
+      SumInduct(m1, k, m[k]); 
+      assert m1[k := m[k]] == m;
+
+      if k in p {
+        SumInduct(p1, k, p[k]); 
+        assert p1[k := p[k]] == p;
+      } else {
+        assert p1 == p;
+      }
+
+      if k in q {
+        SumInduct(q1, k, q[k]); 
+        assert q1[k := q[k]] == q;
+      } else {
+        assert q1 == q;
+      }
+
+      assert forall k :: GetOrZero(p, k) + GetOrZero(q, k) == GetOrZero(m, k)
+          ==> GetOrZero(p1, k) + GetOrZero(q1, k) == GetOrZero(m1, k);
+      SumAdditive(m1, p1, q1);
+
+      assert GetOrZero(p, k) + GetOrZero(q, k) == GetOrZero(m, k);
+    }
+  }
+}
